proof/correctness/Correctness_Mem.ec
@@ -9,6 +9,27 @@ require import XMSS_IMPL.
 require import Utils2. (* valid_ptr predicate *)
 require import Termination.
 
+(** -------------------------------------------------------------------------------------------- **)
+
+lemma or_zero(w0 w1 : W8.t) : 
+    (w0 `|` w1 = W8.zero) <=> (w0 = W8.zero /\ w1 = W8.zero).
+proof.
+split; last first.
+  + move => [-> ->].
+    by rewrite or0w.
+  + rewrite !wordP => H.
+    case (w0 = W8.zero).
+      * move => -> /= k kb. move : (H k kb) => /= /#. 
+      * move => *. have Hk : exists k, 0 <= k < 8 /\ w0.[k]. 
+         - move : (W8.wordP w0 W8.zero); smt(W8.zerowE W8.get_out).
+        elim Hk => k [kb kval]. move : (H k kb). by rewrite orwE kval.
+qed.
+
+lemma xor_eq (w0 w1 : W8.t) :
+    w0 `^` w1 = W8.zero => w0 = w1 by smt(@W8). 
+    
+(** -------------------------------------------------------------------------------------------- **)
+
 (******************************************************************************)
 (******************               MEMSET                          *************)
 (******************************************************************************)
@@ -117,21 +138,6 @@ lemma memset_nseq :
        to_list res = nseq 4 W8.zero] = 1%r
           by conseq memset_zero_ll _memset_nseq; auto.
 
-lemma load_store  (mem : global_mem_t) (ptr : W64.t) (v : W8.t) :
-    loadW8 (storeW8 mem (to_uint ptr) v) (to_uint ptr) = v 
-      by rewrite /storeW8 /loadW8 get_setE ifT.
-
-
-
-
-
-
-
-
-
-
-
-
 lemma memset_ptr_post (ptr : W64.t, len : W64.t, v : W8.t) :
     hoare [M(Syscall).__memset_u8_ptr : 
       0 <= to_uint len < W64.modulus /\
@@ -165,7 +171,6 @@ while (
          admit.
 qed.
 
-
 (******************************************************************************)
 (******************               MEMCPY                          *************)
 (******************************************************************************)
@@ -180,13 +185,28 @@ proof.
 proc.
 inline * ; wp ; sp.
 while (
+  in_ptr1  = ptr /\
+  0 <= (to_uint ptr) + 32 <= W64.modulus /\
+  0 <= to_uint ptr /\
+  
   0 <= i <= 32 /\
   0 <= to_uint in_ptr{hr} + 32 <= W64.modulus /\
   forall (k : int), 0 <= k < i => (out1.[k] = loadW8 Glob.mem ((to_uint ptr) + k))
-) ; auto => />; last first.
-- move => &hr *. split ; 1:smt(@JMemory). move => *. rewrite tP ; smt(@JMemory @Array32).
-- move => &hr *. split ; 1:smt(). move => k *. rewrite get_setE 1:/#. case (k = i{hr}); last by smt(@JMemory).
-  move => E0 ; congr. rewrite E0 to_uintD of_uintK //=. admit. (* overflow *)
+).
+    + auto => /> &hr H0 H1 H2 H3 H4 H5 H6 H7 H8C.
+      do split; 1,2:smt().
+      move => k??.
+      rewrite get_setE //=.
+      case (k = i{hr}) => E.
+          * congr; rewrite E #smt:(@W64 pow2_64).
+          * apply H7 => /#.      
+    + auto => /> &hr H0 H1 H2. 
+      split => [/# | i0 out0 ???]. 
+      have ->: i0 = 32 by smt().
+      move => H3.
+      rewrite tP => j?.
+      rewrite initiE //=. 
+      by apply H3.
 qed.
 
 lemma memcpy_ptr_ll :
@@ -213,38 +233,59 @@ proof.
 by conseq memcpy_ptr_ll (memcpy_ptr_correct ptr).
 qed.
 
-lemma _x_memcpy_u8u8_post (x : W8.t Array32.t) :
-    phoare [M(Syscall)._x_memcpy_u8u8_32_32 : arg.`2 = x ==> res = x] = 1%r.
+lemma _x_memcpy_u8u8_p (x : W8.t Array32.t) :
+hoare [M(Syscall)._x_memcpy_u8u8_32_32 : arg.`2 = x ==> res = x].
 proof.
-proc ; inline*.
-wp ; sp.
-while (* while invariante variante *)
-(0 <= to_uint i <= 32 /\ (forall (k : int), 0 <= k < to_uint i => (out1.[k] = in_01.[k]))) 
-(32 - to_uint i).
-  + auto => /> &hr i *; do split.
-      - smt(@W64).
-      - smt(@W64 pow2_64).
-      - move => k *. rewrite get_setE; 1:smt(@W64). case (k = to_uint i{hr}).
-           * move => * /#. 
-           * move => *. admit.
-      - smt(@W64 pow2_64).
-  + skip => /> &hr *. split; 1:smt(). progress.
-      - smt(@W64).
-      - rewrite tP. smt.
+proc.
+inline.
+wp; sp.
+while (
+  0 <= to_uint i <= 32 /\ 
+  (forall (k : int), 0 <= k < to_uint i => (out1.[k] = in_01.[k])) /\
+
+  in_01 = x
+).
+    + auto => /> &hr H0 H1 H2 H3. 
+      do split; 1,2: by smt(@W64).
+      move => k??.
+      rewrite get_setE 1:#smt:(@W64).
+      case (k = to_uint i{hr}) => [/# | *].
+      apply H2.
+      smt(@W64).
+    + skip => /> &hr.
+      split => [/# | i0 out10 ???].
+      have ->: to_uint i0 = 32 by smt(@W64 pow2_64).
+      by rewrite tP.
 qed.
+
+
+lemma _x_memcpy_u8u8_post (x : W8.t Array32.t) :
+    phoare [
+        M(Syscall)._x_memcpy_u8u8_32_32 : 
+          arg.`2 = x ==> res = x] = 1%r
+            by conseq _x_memcpy_u8u8_32_32_ll (_x_memcpy_u8u8_p x).
 
 lemma _x_memcpy_u8u8_64_ (x : W8.t Array64.t) :
     hoare [M(Syscall)._x_memcpy_u8u8_64_64 : arg.`2 = x ==> res = x].
 proof.
-proc => //=. 
+proc. 
 inline; wp; sp. 
 while (
   in_01 = x /\
   0 <= to_uint i <= 64 /\
   (forall (k : int), 0 <= k < to_uint i => (out1.[k] = x.[k]))
 ).
-    + auto => /> &hr *; do split; 1,2:smt(@W64); move => k *. rewrite get_setE; first by smt(@W64). admit. (* case (k = to_uint i{hr}) ; first by smt(). *)
-    + auto => /> &hr; split; [ smt() | move => *; rewrite tP; smt(@W64 pow2_64) ].
+    + auto => /> &hr H0 H1 H2 H3.
+      do split; 1,2: by smt(@W64). 
+      move => k??. 
+      rewrite get_setE 1:#smt:(@W64).
+      case (k = to_uint i{hr}) => [/# | *].
+      apply H2.
+      smt(@W64).
+    + auto => /> &hr.
+      split => [/# | i0 out10 ???].
+      have ->: to_uint i0 = 64 by smt(@W64 pow2_64).
+      by rewrite tP.
 qed.
 
 
@@ -262,43 +303,40 @@ lemma memcmp_true (x y : W8.t Array32.t) :
         hoare[M(Syscall).__memcmp : arg = (x, y) ==> res = W8.zero].
 proof.
 move => xy_eq.
-proc ; auto => /> *.
+proc.
 while(0 <= to_uint i <= 32 /\ a = b /\ acc = W8.zero) ; auto => /> *; smt(@W64).
-qed.
-
-lemma or_zero(w0 w1 : W8.t) : 
-    (w0 `|` w1 = W8.zero) <=> (w0 = W8.zero /\ w1 = W8.zero).
-proof.
-split; last first.
-  + move => [-> ->].
-    by rewrite or0w.
-  + rewrite !wordP => H.
-    case (w0 = W8.zero).
-      * move => -> /= k kb. move : (H k kb) => /= /#. 
-      * move => *. have Hk : exists k, 0 <= k < 8 /\ w0.[k]. 
-         - move : (W8.wordP w0 W8.zero); smt(W8.zerowE W8.get_out).
-        elim Hk => k [kb kval]. move : (H k kb). by rewrite orwE kval.
 qed.
 
 lemma memcmp_false (x y : W8.t Array32.t) :
     x <> y => 
         hoare[M(Syscall).__memcmp : arg = (x, y) ==> res <> W8.zero].
 proof.
-move => xy_neq.
+move => ?. 
+have E : exists (i : int), 0 <= i < 32 => x.[i] <> y.[i] by smt(@Array32). 
 proc.
-auto => />.
-have E0 : exists (z : int), 0 <= z < 32 => x.[z] <> y.[z] by smt(@Array67).
 while (
   #pre /\
+  (exists (i : int), 0 <= i && i < 32 => x.[i] <> y.[i]) /\
   0 <= to_uint i <= 32 /\ 
-  (exists (k : int), 0 <= k < to_uint i => (a.[k] = b.[k]) => acc <> W8.zero)
-); last first.
-    + auto => />. split; 1:smt(). move => acc i. rewrite /(\ult) of_uintK => ???.
-      have -> : to_uint i = 32 by smt(@W64 pow2_64). move => k ?. admit.
-
-    + auto => /> &r. rewrite !/(\ult) !to_uintD !of_uintK //=. progress;1,2:smt(@W64 pow2_64).
-admit.
+  (acc = W8.zero <=> forall (k : int), 0 <= k < to_uint i => x.[k] = y.[k])
+). 
+    + auto => /> &hr i0???H0. 
+      rewrite ultE of_uintK (: 32 %% W64.modulus = 32) 1:/# => ?. 
+      do split; 1,2: smt(@W64).       
+         * move => H. 
+           have E1 : acc{hr} = W8.zero by smt(or_zero). 
+           have E2 : x.[to_uint i{hr}] `^` y.[to_uint i{hr}] = W8.zero by smt(or_zero).
+           have E3 : x.[to_uint i{hr}] = y.[to_uint i{hr}] by smt(xor_eq).
+           have E4 : forall (k : int), 0 <= k && k < to_uint i{hr} => x.[k] = y.[k] by smt(). 
+           rewrite to_uintD_small /#.
+         * rewrite to_uintD_small 1:/# (: to_uint W64.one = 1) 1:/# => H.
+           rewrite or_zero; split; [rewrite H0 | rewrite H ] => /#.
+    + auto => />; split => [/# | acc0 i0]. 
+      rewrite ultE -lezNgt of_uintK //= => [?i1??? ->].
+      have ->: to_uint i0 = 32 by smt(). 
+      smt(@Array32). 
 qed.
+
 
 (* INLEN = 32 /\ OUTLEN = 2144 *)
 (* pre: copying all elements of in does not write out of bounds in out *)
