proof/correctness/Correctness_WOTS.ec
@@ -19,6 +19,13 @@ require import BitEncoding.
 require import StdBigop. 
 (*---*) import Bigint.
 
+(** -------------------------------------------------------------------------------------------- **)
+
+op load_sig (mem : global_mem_t) (ptr : W64.t) : W8.t Array2144.t =
+  Array2144.init(fun i => loadW8 mem (to_uint ptr + i)).
+
+(** -------------------------------------------------------------------------------------------- **)
+
 lemma nbyte_xor_val (a b : nbytes): 
     val (nbytexor a b) = bytexor (val a) (val b).
 proof.
@@ -33,10 +40,12 @@ lemma zip_fst (a b : W8.t list) (i : int):
     (nth witness (zip a b) i).`1 = nth witness a i 
       by smt(@List).
 
-lemma zip_snd (a b : W8.t list) (i : int):
+lemma zip_snd (a b : W8.t list) (i : int) :
   0 <= i < min (size a) (size b) =>
-    (nth witness (zip a b) i).`2 = nth witness b i 
-      by smt(@List).
+    (nth witness (zip a b) i).`2 = nth witness b i
+       by smt(@List).
+
+(** -------------------------------------------------------------------------------------------- **)
 
 lemma base_w_correctness_64 ( _in_ : W8.t Array32.t) :
     floor (log2 w%r) = XMSS_WOTS_LOG_W /\ 
@@ -67,7 +76,6 @@ while (
   _in{2} = to_uint in_0{1} /\ _in{2} = (consumed{2} + 1) %/ 2 /\
   (forall (j : int), 0 <= j < to_uint out{1} => (to_uint output{1}.[j]) = nth witness base_w{2} j)
 ).
-(* First subgoal of while *)
     + if.
         * auto => /> &1 &2 *; smt(@W64).
         * admit. (* auto => /> &1 &2 *; do split;1..11:smt(@W64 @IntDiv pow2_64 size_put).
@@ -95,7 +103,6 @@ while (
                   rewrite and_mod //= to_uint_truncateu8 to_uint_zeroextu32 //=. 
                   rewrite to_uintB 1:#smt:(@W64) //=. 
                   admit. (* smt(@W64 @W8 @W32 pow2_32 pow2_64 pow2_8 @IntDiv). *) (* This call to smt fails sometimes *)
-(* Last subgoal of while *)
     + skip => /> *; do split;2,3:smt(@W64 pow2_64). by rewrite size_nseq.
 qed.
 
@@ -144,7 +151,6 @@ while (
   _in{2} = to_uint in_0{1} /\ _in{2} = (consumed{2} + 1) %/ 2 /\
   (forall (j : int), 0 <= j < to_uint out{1} => (to_uint output{1}.[j]) = nth witness base_w{2} j)
 ).
-(* First subgoal of while *)
     + if.
         * auto => /> &1 &2 *; smt(@W64).
         * auto => /> &1 &2 *; do split;1..11:smt(@W64 @IntDiv pow2_64 size_put).
@@ -171,7 +177,6 @@ while (
                   rewrite and_mod //= to_uint_truncateu8 to_uint_zeroextu32 //=. 
                   rewrite to_uintB 1:#smt:(@W64) //=. 
                   admit. (* smt(@W64 @W8 @W32 pow2_32 pow2_64 pow2_8 @IntDiv). *) (* this call to smt fails sometimes *)
-(* Last subgoal of while *)
     + skip => /> *; do split;2,3:smt(@W64 pow2_64). by rewrite size_nseq.
 qed.
 
@@ -190,6 +195,8 @@ proof.
 move => [#] ??. 
 admit.
 qed.
+
+(** -------------------------------------------------------------------------------------------- **)
 
 lemma wots_checksum_correctness (msg : W32.t Array64.t) :
     len1 = XMSS_WOTS_LEN1 /\  w = XMSS_WOTS_W =>
@@ -233,7 +240,10 @@ proof.
 admit.
 qed.
 
-lemma gen_chain_inplace_correct (_buf_ : W8.t Array32.t, _start_ _steps_ : W32.t, _addr_ : W32.t Array8.t, _pub_seed_ : W8.t Array32.t) :
+(** -------------------------------------------------------------------------------------------- **)
+
+lemma gen_chain_inplace_correct (_buf_ : W8.t Array32.t, _start_ _steps_ : W32.t, 
+                                 _addr_ : W32.t Array8.t, _pub_seed_ : W8.t Array32.t) :
     n = XMSS_N /\
     w = XMSS_WOTS_W /\ 
     len = XMSS_WOTS_LEN /\
@@ -243,7 +253,8 @@ lemma gen_chain_inplace_correct (_buf_ : W8.t Array32.t, _start_ _steps_ : W32.t
     equiv [
       M(Syscall).__gen_chain_inplace ~ Chain.chain : 
       arg{1}= (_buf_, _start_, _steps_, _pub_seed_, _addr_) /\
-      arg{2} = (NBytes.insubd (to_list _buf_), to_uint _start_, to_uint _steps_, NBytes.insubd (to_list _pub_seed_), _addr_) /\
+      arg{2} = (NBytes.insubd (to_list _buf_), to_uint _start_, to_uint _steps_, 
+                NBytes.insubd (to_list _pub_seed_), _addr_) /\
       0 <= to_uint _start_ <= XMSS_WOTS_W - 1/\
       0 <= to_uint _steps_ <= XMSS_WOTS_W - 1 /\
       0 <= to_uint (_start_ + _steps_) <= XMSS_WOTS_W - 1  
@@ -301,7 +312,8 @@ seq 27 9 : (
   buf{2} = to_list buf{1} /\ 
   addr2{1} = address{2}
 ); last first.
-    + inline {1} M(Syscall).__core_hash__96 M(Syscall)._core_hash_96; wp; sp; ecall {1} (hash_96 in_00{1}); auto => /> *. 
+    + inline {1} M(Syscall).__core_hash__96 M(Syscall)._core_hash_96; wp; sp.
+      ecall {1} (hash_96 in_00{1}); auto => /> *. 
       do split; 3..5,8,9:smt(@W32 pow2_32); smt().
 seq 17 1 : (
   #pre /\ 
@@ -312,12 +324,10 @@ seq 17 1 : (
 ); first by ecall {1} (addr_to_bytes_correctness addr{1}); auto => /> /#. 
 swap {2} 7 -6.
 seq 2 1 : (#pre /\ padding{2} = to_list padding{1}); first by call {1} (ull_to_bytes_32_correct W64.zero); auto => /> /#.
-
 seq 1 0 : (
   #pre /\
   (forall (k : int), 0 <= k < 32 => buf{1}.[k] = padding{1}.[k])
 ); first by auto => /> *; smt(@Array96).
-
 seq 1 1 : (
   #pre /\ 
   val _key{2} = to_list aux{1}
@@ -377,8 +387,8 @@ while{1}  (
 ) (32 - to_uint i0{1}). 
     + auto => /> &hr *; do split;3,4,6:smt(@W64 pow2_64).
         * move => *. rewrite get_setE 1:#smt:(@W64) ifF 1:#smt:(@W64 pow2_64) #smt:(@Array96).
-        * move => *. rewrite get_setE 1:#smt:(@W64) ifF 1:#smt:(@W64 pow2_64) #smt:(@Array96).
-        * move => k *. rewrite get_setE 1:#smt:(@W64). 
+        * move => *. rewrite get_setE 1:#smt:(@W64) ifF 1:#smt:(@W64 pow2_64) #smt:(@Array96). (* this smt fails sometimes *)
+        * move => k *. rewrite get_setE 1:#smt:(@W64). (* this smt fails sometimes *)
           case (64 + k = to_uint ((of_int 64)%W64 + i0{hr})); [move => ?; do congr |]; smt(@W64 pow2_64).
     + auto => /> &1 &2. 
       move => H0 H1 H2 H3 H4 H5 H6 H7 H8 H9.
@@ -417,6 +427,8 @@ while{1}  (
       rewrite zip_snd; [rewrite !size_to_list /# |]. 
       rewrite !get_to_list /#. 
 qed.
+
+(** -------------------------------------------------------------------------------------------- **)
 
 lemma expand_seed_correct (_in_seed _pub_seed : W8.t Array32.t, _addr : W32.t Array8.t) :
     len = XMSS_WOTS_LEN /\ 
@@ -547,6 +559,8 @@ proof.
 admit. (* correctness & wots_sk_size from properties *)
 qed.
 
+(** -------------------------------------------------------------------------------------------- **)
+
 lemma pkgen_correct (_seed_ _pub_seed_ : W8.t Array32.t, _addr_ : W32.t Array8.t) :
     w = XMSS_WOTS_W /\
     len = XMSS_WOTS_LEN /\
@@ -647,7 +661,8 @@ auto => /> &1 &2 H0 H1 H2 H3 H4 H5 H6 H7 H8 H9; do split;2,3,6,7:smt().
           * rewrite (nth_flatten witness 32). 
               - pose P := (fun (s : W8.t list) => size s = 32).
                 pose L := (map NBytes.val (put pk{2} i{2} pk_i{2})).
-                rewrite -(all_nthP P L witness) /L size_map size_put H2 => j Hj.                    rewrite /P (nth_map witness); [by rewrite size_put H2 |].       
+                rewrite -(all_nthP P L witness) /L size_map size_put H2 => j Hj.   
+                rewrite /P (nth_map witness); [by rewrite size_put H2 |].       
                 rewrite nth_put 1:/# #smt:(NBytes.valP).
             rewrite map_put nth_put; [rewrite size_map /# |].
             rewrite ifT 1:/# -H9 get_to_list /#.
@@ -671,10 +686,7 @@ move => k??.
 rewrite /DecodeWotsSk /of_list initiE 1:/# => />.
 qed.
 
-(*** Pk From Sig : Doing ***)
-
-op load_sig (mem : global_mem_t) (ptr : W64.t) : W8.t Array2144.t =
-  Array2144.init(fun i => loadW8 mem (to_uint ptr + i)).
+(** -------------------------------------------------------------------------------------------- **)
 
 lemma pk_from_sig_correct (mem : global_mem_t) (_sig_ptr_ : W64.t, _msg_ _pub_seed_ : W8.t Array32.t, _addr_ : W32.t Array8.t) :
     valid_ptr_i _sig_ptr_ 2144 =>
@@ -694,47 +706,47 @@ lemma pk_from_sig_correct (mem : global_mem_t) (_sig_ptr_ : W64.t, _msg_ _pub_se
       arg{1}.`4 = _pub_seed_ /\ 
       arg{1}.`5 = _addr_ /\ 
       Glob.mem{1} = mem /\
-      arg{2} = (to_list _msg_, EncodeWotsSignature (load_sig mem _sig_ptr_), to_list _pub_seed_, _addr_) /\
+      arg{2} = (NBytes.insubd (to_list _msg_), EncodeWotsSignature (load_sig mem _sig_ptr_), NBytes.insubd (to_list _pub_seed_), _addr_) /\
       Glob.mem{2} = mem
       ==>
       res{1}.`1 = DecodeWotsPk res{2}.`1 /\ 
       res{1}.`2 = res{2}.`2
     ].
 proof.
-rewrite /XMSS_N /XMSS_WOTS_LOG_W /XMSS_WOTS_W /XMSS_WOTS_LEN1 /XMSS_WOTS_LEN2.
-move => ? [#] n_val logw_val w_val len1_val len2_val *.
+rewrite /XMSS_N /XMSS_WOTS_LOG_W /XMSS_WOTS_W /XMSS_WOTS_LEN1 /XMSS_WOTS_LEN2 /XMSS_WOTS_LEN.
+move => ? [#] n_val logw_val w_val len1_val len2_val len_val *.
 proc; auto => />. 
 conseq (: _ ==> 
   address{2} = addr{1} /\ 
-  forall (k : int), 0 <= k < 2144 => pk{1}.[k] = nth witness (flatten tmp_pk{2}) k
-); first by auto => /> *; rewrite /DecodeWotsPk /of_list tP; smt(@Array2144).
-
+  size tmp_pk{2} = len /\
+  forall (k : int), 0 <= k < 2144 => pk{1}.[k] = nth witness (nbytes_flatten tmp_pk{2}) k
+).
+    + auto => /> pkL pkR H0 H1 *.
+      rewrite /DecodeWotsPk insubdK; [by rewrite /P H0 |].
+      rewrite tP => i?.
+      rewrite /of_list initiE //=. 
+      by apply H1.
 seq 1 1 : (
   sig_ptr{1} = _sig_ptr_ /\
   addr{1} = address{2} /\
-  M{2} = to_list msg{1} /\
-  _seed{2} = to_list pub_seed{1} /\
+  val M{2} = to_list msg{1} /\
+  val _seed{2} = to_list pub_seed{1} /\
   sig{2} = EncodeWotsSignature (load_sig mem sig_ptr{1}) /\
 
   size tmp_pk{2} = 67 /\
-  (forall (t : W8.t list), t \in tmp_pk{2} => size t = 32) /\
 
   Glob.mem{1} = mem /\ Glob.mem{2} = mem /\
   valid_ptr_i sig_ptr{1} 2144
-); first by auto => />; split; [by rewrite size_nseq /# | smt(@List)].
-
+).
+    + auto => />. 
+      do split; 1,2: by rewrite insubdK //= /P size_to_list n_val.
+      by rewrite size_nseq len_val /#. 
 inline M(Syscall).__chain_lengths_ M(Syscall)._chain_lengths M(Syscall).__chain_lengths.
-
 seq 11 0 : (#pre /\ lengths2{1} = lengths{1} /\ msg2{1} = msg{1}); first by auto.
-
 seq 1 1 : (
-  M{2} = to_list msg{1} /\
-  _seed{2} = to_list pub_seed{1} /\
+  val M{2} = to_list msg{1} /\
+  val _seed{2} = to_list pub_seed{1} /\
   address{2} = addr{1} /\
-  size sig{2} = 67 /\
-  size (flatten sig{2}) = 2144 /\
-  (forall (t : W8.t list), t \in sig{2} => size t = 32) /\ 
-  size M{2} = 32 /\
   sig{2} = EncodeWotsSignature (load_sig mem sig_ptr{1}) /\
   lengths2{1} = lengths{1} /\ 
 
@@ -742,28 +754,19 @@ seq 1 1 : (
   (forall (k : int), 0 <= k < 64 => 0 <= to_uint t0{1}.[k] < w) /\
 
   size tmp_pk{2} = 67 /\
-  (forall (t : W8.t list), t \in tmp_pk{2} => size t = 32) /\
   
-
-  Glob.mem{1} = mem /\ Glob.mem{2} = mem /\
+  Glob.mem{1} = mem /\ 
+  Glob.mem{2} = mem /\
   valid_ptr_i sig_ptr{1} 2144
 ).
     + exists * msg2{1}; elim * => P; call (base_w_results_64 P) => //=.
-      skip => /> *; do split.
-         * rewrite /EncodeWotsSignature size_chunk //= size_to_list //.
-         * rewrite /EncodeWotsSignature size_flatten sumzE BIA.big_map /(\o) //= -(StdBigop.Bigint.BIA.eq_big_seq (fun _ => 32)) 1:#smt:(@List @BitChunking).
-           rewrite  big_constz count_predT size_chunk //= size_to_list //=.  
-         * rewrite /EncodeWotsSignature => />; smt(@List @BitChunking).
-         * by rewrite size_to_list. 
-
+      auto => /> *. 
+      smt().
 seq 2 0 : (
-  M{2} = to_list msg{1} /\
-  _seed{2} = to_list pub_seed{1} /\
+  val M{2} = to_list msg{1} /\
+  val _seed{2} = to_list pub_seed{1} /\
   address{2} = addr{1} /\
-  size sig{2} = 67 /\
-  size (flatten sig{2}) = 2144 /\
-  (forall (t2 : W8.t list), t2 \in sig{2} => size t2 = 32) /\
-  size M{2} = 32 /\
+  
   sig{2} = EncodeWotsSignature (load_sig mem sig_ptr{1}) /\
   msg{2} = map W32.to_uint (to_list t0{1}) /\
   (forall (k : int), 0 <= k < 64 => 0 <= to_uint t0{1}.[k] < w) /\
@@ -771,49 +774,41 @@ seq 2 0 : (
   (forall (k : int), 0 <= k < 64 => to_uint lengths2{1}.[k] = nth witness msg{2} k) /\
 
   size tmp_pk{2} = 67 /\
-  (forall (t : W8.t list), t \in tmp_pk{2} => size t = 32) /\
-  
 
-  Glob.mem{1} = mem /\ Glob.mem{2} = mem /\
+  Glob.mem{1} = mem /\ 
+  Glob.mem{2} = mem /\
   valid_ptr_i sig_ptr{1} 2144
 ).
     + auto => /> *.
       rewrite (nth_map witness); [by rewrite size_to_list |].
       rewrite initiE 1:/# => />. 
-      rewrite ifT //=.  
-
+      by rewrite ifT.  
 inline {1} M(Syscall).__wots_checksum.
 seq 5 0 : (#pre /\ csum_base_w{1} = t1{1} /\ msg_base_w{1} = lengths2{1}); first by auto.
-
 seq 1 0 : (
   #pre /\
   (forall (k : int), 0 <= k < 64 => 0 <= to_uint buf{1}.[k] < w) /\
   msg{2} = map (W32.to_uint) (to_list buf{1})
 ).
-    + auto => /> &1 &2 ????? H4 *; do split => [ * |]. do split.
-          - rewrite initiE //= H4 // (nth_map witness); [ by rewrite size_to_list //= |].
+    + auto => /> &1 &2 H0 H1 H2 H3 H4 H5 H6; do split => [ k?? |]. 
+      do split.
+          - rewrite initiE //= H3// (nth_map witness); [ by rewrite size_to_list //= |].
             rewrite get_to_list /#.
-          - rewrite initiE //= H4 //= (nth_map witness); [ by rewrite size_to_list //= |].
+          - rewrite initiE //= H3 //= (nth_map witness); [ by rewrite size_to_list //= |].
             rewrite get_to_list /#.
           - apply (eq_from_nth witness); [ by rewrite !size_map !size_iota |].
             rewrite size_map size_to_list => i Hi.
-            rewrite -H4 //= (nth_map witness); [ by rewrite size_to_list |]. 
+            rewrite -H3 //= (nth_map witness); [ by rewrite size_to_list |]. 
             rewrite get_to_list //= initiE //=.
-
 seq 1 1 : (#pre /\ to_uint csum{1} = csum{2} /\ 0 <= csum{2} <= len1 * (w - 1)).
     + exists * buf{1}; elim * => P; call {1} (wots_checksum_results P) => //.
       skip => /> /#.
-
 seq 3 0 : (#pre /\ u{1} = W64.of_int 4); first by auto.
-
 seq 2 2 : (
-  M{2} = to_list msg{1} /\
-  _seed{2} = to_list pub_seed{1} /\
+  val M{2} = to_list msg{1} /\
+  val _seed{2} = to_list pub_seed{1} /\
   address{2} = addr{1} /\
-  size sig{2} = 67 /\
-  size (flatten sig{2}) = 2144 /\
-  (forall (t2 : W8.t list), t2 \in sig{2} => size t2 = 32) /\
-  size M{2} = 32 /\
+  
   sig{2} = EncodeWotsSignature (load_sig mem sig_ptr{1}) /\
   msg{2} = map W32.to_uint (to_list t0{1}) /\
   
@@ -828,43 +823,36 @@ seq 2 2 : (
 
   to_uint csum{1} = to_uint csum_32{2} /\
 
-
   size tmp_pk{2} = 67 /\
-  (forall (t : W8.t list), t \in tmp_pk{2} => size t = 32) /\
-  
 
-  Glob.mem{1} = mem /\ Glob.mem{2} = mem /\
+  Glob.mem{1} = mem /\ 
+  Glob.mem{2} = mem /\
   valid_ptr_i sig_ptr{1} 2144
 ).
     + auto => /> &1 &2 *. 
       rewrite (: 63 = 2^6 - 1) 1:/# and_mod //=. 
       have ->: truncateu8 ((of_int 4))%W64 = W8.of_int 4 by smt(@W64 pow2_64).
       rewrite !shl_shlw //= len2_val w_val.
-      have ->: floor (log2 16%r) = 4 by rewrite log2_16 from_int_floor.
-      by simplify.
-      have ->: floor (log2 16%r) = 4 by rewrite log2_16 from_int_floor.
-      simplify.
+        * (have ->: floor (log2 16%r) = 4 by rewrite log2_16 from_int_floor) => //=.
+      (have ->: floor (log2 16%r) = 4 by rewrite log2_16 from_int_floor) => //=.
       rewrite !to_uint_shl //= of_uintK //=.
       have ->: to_uint csum{1} %% 4294967296 = to_uint csum{1} by smt(@W64 pow2_64 @IntDiv).
-      smt(@IntDiv).
-
+      smt(modz_small).
 seq 0 1 : (#pre /\ len_2_bytes{2} = 2).
     + auto => /> *. 
-      rewrite w_val len2_val log2_16 -fromintM //= from_int_ceil //=; apply ceil_3_2.
-
+      rewrite w_val len2_val log2_16 -fromintM //= from_int_ceil //=.
+      apply ceil_3_2.
 seq 1 1 : (#pre /\ to_list csum_bytes_p{1} = csum_bytes{2}).
     + ecall {1} (ull_to_bytes_2_equiv csum{1}). 
-      auto => /> &1 &2 H0 H1 H2 H3 H4 H5 H6 H7 H8 H9 H10 H11 H12 H13 H14 rL H15 *.
-      rewrite H15 //=; congr; smt(@W32). 
-
+      auto => /> &1 &2 ????????????? H. 
+      rewrite H //=.
+      congr. 
+      smt(@W32). 
 seq 1 1 : (
-  M{2} = to_list msg{1} /\
-  _seed{2} = to_list pub_seed{1} /\
+  val M{2} = to_list msg{1} /\
+  val _seed{2} = to_list pub_seed{1} /\
   address{2} = addr{1} /\
-  size sig{2} = 67 /\
-  size (flatten sig{2}) = 2144 /\
-  (forall (t2 : W8.t list), t2 \in sig{2} => size t2 = 32) /\
-  size M{2} = 32 /\
+  
   sig{2} = EncodeWotsSignature (load_sig mem sig_ptr{1}) /\
   msg{2} = map W32.to_uint (to_list t0{1}) /\
   
@@ -890,22 +878,19 @@ seq 1 1 : (
   (forall (k : int), 0 <= k < 3 => 0 <= to_uint csum_base_w{1}.[k] < w) /\
 
   size tmp_pk{2} = 67 /\
-  (forall (t : W8.t list), t \in tmp_pk{2} => size t = 32) /\
 
-  Glob.mem{1} = mem /\ Glob.mem{2} = mem /\
+  Glob.mem{1} = mem /\ 
+  Glob.mem{2} = mem /\
   valid_ptr_i sig_ptr{1} 2144
 ).
     + exists * csum_bytes_p{1}; elim * => P; call (base_w_results_3 P) => //=.
-      auto => /> *; smt(array3_map_bounds).
-
+      auto => /> *. 
+      smt(array3_map_bounds).
 seq 6 1 : (
-  M{2} = to_list msg{1} /\
-  _seed{2} = to_list pub_seed{1} /\
+  val M{2} = to_list msg{1} /\
+  val _seed{2} = to_list pub_seed{1} /\
   address{2} = addr{1} /\
-  size sig{2} = 67 /\
-  size (flatten sig{2}) = 2144 /\
-  (forall (t2 : W8.t list), t2 \in sig{2} => size t2 = 32) /\
-  size M{2} = 32 /\
+  
   sig{2} = EncodeWotsSignature (load_sig mem sig_ptr{1}) /\
   
   0 <= csum{2} <= len1 * (w - 1) /\
@@ -919,12 +904,12 @@ seq 6 1 : (
   (forall (k : int), 0 <= k < 67 => 0 <= to_uint lengths{1}.[k] < w) /\
   
   size tmp_pk{2} = 67 /\
-  (forall (t : W8.t list), t \in tmp_pk{2} => size t = 32) /\
 
-  Glob.mem{1} = mem /\ Glob.mem{2} = mem /\
+  Glob.mem{1} = mem /\ 
+  Glob.mem{2} = mem /\
   valid_ptr_i sig_ptr{1} 2144
 ).
-    + auto => /> &1 &2 ????? H5 * ; do split.
+    + auto => /> &1 &2 ?? H0 H1 ? H5 * ; do split.
         * apply (eq_from_nth witness); [ rewrite size_cat !size_map !size_iota //= |].
           rewrite size_map size_to_list => i?.
           rewrite nth_cat !size_map size_iota (: max 0 64 = 64) 1:/#. 
@@ -932,16 +917,17 @@ seq 6 1 : (
               - move => ?.  
                 rewrite ifT 1:/# (nth_map witness); [by rewrite size_to_list |]. 
                 rewrite get_to_list initiE 1:/# => />.  
-                rewrite ifF 1:/# H5 //=.
+                rewrite ifF 1:/# H5 //= /#.
               - move => ?. 
                 rewrite ifF 1:/# (nth_map witness); [ by rewrite size_to_list |]. 
                 rewrite get_to_list initiE 1:/# => />. 
-                rewrite ifT 1:/# (nth_map witness); [ by rewrite size_to_list /# |]. 
+                rewrite ifT 1:/# (nth_map witness); [ by rewrite size_to_list /# |].
                 rewrite get_to_list //=. 
         * move => k??; do split.             
               - rewrite initiE 1:/# => />.
                 case (0 <= k < 64).  
-                    + move => ?. rewrite ifF 1:/# H5 //=.  
+                    + move => ?. 
+                      rewrite ifF 1:/# H1 //=.
                       rewrite (nth_map witness); [ by rewrite size_to_list |]. 
                       rewrite get_to_list /#. 
                     + move => ?; rewrite ifT /#.
@@ -949,7 +935,7 @@ seq 6 1 : (
                 rewrite initiE //=.
                 case (0 <= k < 64).  
                     + move => ?. 
-                      rewrite ifF 1:/# H5 //.  
+                      rewrite ifF 1:/# H1 //.  
                       rewrite (nth_map witness); [ by rewrite size_to_list |]. 
                       rewrite get_to_list /#. 
                     + move => ?; rewrite ifT /#.
@@ -959,11 +945,9 @@ while (
   ={i} /\ 
   0 <= i{1} <= 67 /\
   #pre /\
-  (forall (k : int), 0 <= k < 32 * i{1} => pk{1}.[k] = nth witness (flatten tmp_pk{2}) k) (* parte consumida *)
+  (forall (k : int), 0 <= k < 32 * i{1} => pk{1}.[k] = nth witness (nbytes_flatten tmp_pk{2}) k) (* parte consumida *)
 ); last by auto => /> /#.
-
 seq 2 1 : (#pre); first by inline{1}; auto.
-
 seq 1 1 : (
   #pre /\ 
   start{1} = lengths{1}.[i{1}] /\
@@ -972,83 +956,119 @@ seq 1 1 : (
   0 <= to_uint start{1} < w
 ).
     + auto => /> &1 &2 *; rewrite (nth_map witness); [ by rewrite size_to_list |]. 
-      rewrite get_to_list //= /#. 
- 
+      rewrite get_to_list //= /#.  
 seq 4 0 : (
   #pre /\ 
   steps{1} = (W32.of_int 15) - lengths{1}.[i{2}] /\
   0 <= to_uint (start{1} + steps{1}) < w /\
   t{1} = sig_ptr{1} + W64.of_int (i{1} * 32)
 ).
-
-auto => /> &1 &2 H0 H1 H2 H3 H4 H5 H6 H7 H8 H9 H10 H11 H12 H13 *; do split => [| ?].
-    * rewrite to_uintD ; smt(@W32 pow2_32). 
-    * have ->: lengths{1}.[i{2}] + ((of_int 15)%W32 - lengths{1}.[i{2}]) =  (of_int 15)%W32 by ring. 
-      rewrite of_uintK w_val //=. 
-
+    + auto => /> &1 &2 *; do split => [| ?].
+        * rewrite to_uintD #smt:(@W32 pow2_32). 
+        * have ->: lengths{1}.[i{2}] + ((of_int 15)%W32 - lengths{1}.[i{2}]) =  (of_int 15)%W32 by ring. 
+          rewrite of_uintK w_val //=. 
 seq 1 1 : (
   #pre /\
-  to_list aux_0{1} = sig_i{2}
+  to_list aux_0{1} = val sig_i{2}
 ). 
     + exists * t{1} ; elim * => P.
       ecall {1} (p_memcpy_ptr_correct P).
       auto => /> &1 &2 *; do split; 1..3: smt(@W64 pow2_64).
       move => *. 
       rewrite /EncodeWotsSignature /load_sig; apply (eq_from_nth witness). 
-          * rewrite size_to_list size_nth_chunk //= size_to_list /#. 
+          * rewrite size_to_list valP /#.  
           * rewrite size_to_list => i? />. 
-            rewrite initiE //= /chunk nth_mkseq; [by rewrite size_to_list /# |] => />. 
-            rewrite nth_take //= 1:/# nth_drop 1,2:/# get_to_list initiE 1:/# => />.                
-            congr; smt(@W64 pow2_64). 
-(*** tou aqui **)
+            rewrite initiE //= /chunk size_to_list.  
+            rewrite insubdK; [rewrite /P size_map size_mkseq /# |].
+            rewrite (nth_map witness); [rewrite size_mkseq /# |].
+            rewrite insubdK.  
+                 - rewrite /P nth_mkseq 1:/# => />.
+                   rewrite size_take 1:/# size_drop 1:/# !size_to_list /#.                     
+            rewrite nth_mkseq 1:/# => />.
+            rewrite nth_take 1,2:/# nth_drop 1,2:/# get_to_list initiE 1:/# => />. 
+            congr. 
+            smt(@W64 pow2_64).
 seq 2 1 : (
     ={i} /\
     0 <= i{1} && i{1} <= 67 /\
-M{2} = to_list msg{1} /\
-_seed{2} = to_list pub_seed{1} /\
-address{2} = addr{1} /\
-size sig{2} = 67 /\
-size (flatten sig{2}) = 2144 /\
-(forall (t2 : W8.t list), t2 \in sig{2} => size t2 = 32) /\
-size M{2} = 32 /\
-sig{2} = EncodeWotsSignature (load_sig mem sig_ptr{1}) /\
-(0 <= csum{2} && csum{2} <= len1 * (w - 1)) /\
-to_uint csum{1} = to_uint csum_32{2} /\
-to_list csum_bytes_p{1} = csum_bytes{2} /\
--csum_base_w{2} = map W32.to_uint (to_list csum_base_w{1}) /\
-(forall (k0 : int), 0 <= k0 < 3 => 0 <= to_uint csum_base_w{1}.[k0] < w) /\
-map W32.to_uint (to_list lengths{1}) = msg{2} /\
-(forall (k0 : int), 0 <= k0 < 67 => 0 <= to_uint lengths{1}.[k0] < w) /\
-Glob.mem{1} = mem /\ 
-Glob.mem{2} = mem /\ 
-valid_ptr_i sig_ptr{1} 2144 /\
-(forall (k0 : int), 0 <= k0 < 32 * i{1} => pk{1}.[k0] = nth witness (flatten tmp_pk{2}) k0) /\
-i{1} < 67 /\ 
-i{2} < len /\
-    to_list aux_0{1} = pk_i{2} /\
-    aux_1{1} = address{2}
+    val M{2} = to_list msg{1} /\
+    val _seed{2} = to_list pub_seed{1} /\
+    sig{2} = EncodeWotsSignature (load_sig mem sig_ptr{1}) /\
+    (0 <= csum{2} && csum{2} <= len1 * (w - 1)) /\
+    to_uint csum{1} = to_uint csum_32{2} /\
+    to_list csum_bytes_p{1} = csum_bytes{2} /\
+    csum_base_w{2} = map W32.to_uint (to_list csum_base_w{1}) /\
+    (forall (k0 : int), 0 <= k0 < 3 => 0 <= to_uint csum_base_w{1}.[k0] < w) /\
+    map W32.to_uint (to_list lengths{1}) = msg{2} /\
+    (forall (k0 : int), 0 <= k0 < 67 => 0 <= to_uint lengths{1}.[k0] < w) /\
+    Glob.mem{1} = mem /\ 
+    Glob.mem{2} = mem /\ 
+    valid_ptr_i sig_ptr{1} 2144 /\
+    (forall (k0 : int), 0 <= k0 < 32 * i{1} => pk{1}.[k0] = nth witness (nbytes_flatten tmp_pk{2}) k0) /\
+    i{1} < 67 /\ 
+    i{2} < len /\
+    to_list aux_0{1} = val pk_i{2} /\
+    aux_1{1} = address{2} /\
+    size tmp_pk{2} = 67
 ).
-    + inline M(Syscall).__gen_chain_inplace_ M(Syscall)._gen_chain_inplace; wp; sp. 
+    + inline M(Syscall).__gen_chain_inplace_ M(Syscall)._gen_chain_inplace.
+      wp; sp. 
       exists * out0{1}, start0{1}, steps0{1}, addr1{1}, pub_seed1{1}.  
-      elim * => _P1 _P2 _P3 _P4 _P5 *.  
-      call (gen_chain_inplace_correct _P1 _P2 _P3 _P4 _P5) => [/# |].
-      skip => /> &1 &2 *; do split; first last.
-          * admit.
-          * smt(). 
-          * smt(@W32 pow2_32). 
-          * admit. 
-          * smt(@W32 pow2_32). 
-          * move => [#] *; split. admit. admit.
-          * apply (eq_from_nth witness); rewrite !size_to_list //= => i?.
-            admit. 
-
-auto => /> &1 &2 *; do split;1,2,4,5:smt(). 
-move => k0??.
-rewrite initiE 1:/# => />. 
-rewrite (nth_flatten witness 32).
-    + rewrite size_all_r; apply all_put => />; [ by rewrite size_to_list |]. admit. 
-case: (i{2} * 32 <= k0 && k0 < i{2} * 32 + 32) => H.
-  + rewrite nth_put. admit. rewrite ifT 1:/# get_to_list /#. 
-  + rewrite nth_put. admit. rewrite ifF 1:/# -nth_flatten. admit.  smt(). 
+      elim * => P0 P1 P2 P3 P4 P5.  
+      call (gen_chain_inplace_correct P0 P1 P2 P3 P4) => [/# |]. 
+      auto => /> &1 &2 H0 H1 H2 H3 H4 H5 H6 H7 H8 H9 H10 H11 H12 H13 H14 H15 H16 H17 H18 H19*.
+      do split.
+         * apply nbytes_eq.
+           apply (eq_from_nth witness); first by rewrite !NBytes.valP.
+           rewrite NBytes.valP n_val => j?.
+           rewrite -H19 get_to_list insubdK; [by rewrite /P size_to_list n_val |]. 
+           rewrite get_to_list initiE //= initiE 1:/# => />. 
+           rewrite ifT /#.
+         * rewrite w_val //= to_uintB 1:#smt:(@W32 pow2_32) of_uintK //=.
+         * rewrite -H3 #smt:(@NBytes). 
+         * smt().
+         * rewrite to_uintB 1:#smt:(@W32 pow2_32) of_uintK //= /#.
+         * move => ?. 
+           rewrite to_uintB 1:#smt:(@W32 pow2_32) of_uintK //= /#.
+         * smt().
+         * move => *.
+           split => [k0?? | /#]. 
+           rewrite initiE 1:/# => />. 
+           rewrite ifF 1:/#. 
+           by apply H12.
+    + auto => /> &1 &2 H0 H1 H2 H3 H4 H5 H6 H7 H8 H9 H10 H11 H12 H13 H14 H15 *. 
+      do split. 
+          - smt().
+          - smt().
+          - by rewrite size_put. 
+          - move => k??. 
+            rewrite initiE 1:/# => />.
+            case (i{2} * 32 <= k && k < i{2} * 32 + 32) => *.
+               * rewrite /nbytes_flatten (nth_flatten witness 32). 
+                   - pose P := (fun (s : W8.t list) => size s = 32).
+                     pose L := (map NBytes.val (put tmp_pk{2} i{2} pk_i{2})).
+                     rewrite -(all_nthP P L witness). 
+                     rewrite /L /P size_map size_put H15 => j?. 
+                     rewrite (nth_map witness); [ by rewrite size_put H15 |]. 
+                     smt(NBytes.valP). 
+                 rewrite (nth_map witness) 1:#smt:(size_put) nth_put 1:/# ifT 1:/#.
+                 rewrite -H14 get_to_list /#.
+               * rewrite /nbytes_flatten (nth_flatten witness 32). 
+                   - pose P := (fun (s : W8.t list) => size s = 32).
+                     pose L := (map NBytes.val (put tmp_pk{2} i{2} pk_i{2})).
+                     rewrite -(all_nthP P L witness). 
+                     rewrite /L /P size_map size_put H15 => j?. 
+                     rewrite (nth_map witness); [ by rewrite size_put H15 |]. 
+                     smt(NBytes.valP).       
+                 rewrite (nth_map witness) 1:#smt:(size_put) nth_put 1:/# ifF 1:/#.
+                 rewrite H11 1:/# /nbytes_flatten (nth_flatten witness 32).
+                   - pose P := (fun (s : W8.t list) => size s = 32).
+                     pose L := (map NBytes.val tmp_pk{2}).
+                     rewrite -(all_nthP P L witness). 
+                     rewrite /L /P size_map H15 => j?. 
+                 rewrite (nth_map witness) 1:/# #smt:(NBytes.valP).
+                 by rewrite (nth_map witness) 1:/#.
+          - smt().
+          - smt().
 qed.
-        
+
