proof/correctness/Utils2.ec
@@ -1,12 +1,21 @@
 pragma Goals : printall.
 
 require import AllCore List RealExp IntDiv.
+
 require import BitEncoding.
 (*---*) import BitChunking.
 
 from Jasmin require import JModel.
 
 require import Params.
+
+require import Array3.
+
+(** -------------------------------------------------------------------------------------------- **)
+
+lemma nbyte_list_val_eq (a : W8.t list) (b :nbytes) : 
+    size a = n => NBytes.insubd a = b => val b = a by 
+      smt(@NBytes).
 
 (** -------------------------------------------------------------------------------------------- **)
 
@@ -23,3 +32,43 @@ pred valid_ptr_i (p : W64.t) (o : int) =
 lemma nbytes_eq:
   forall (s1 s2 : nbytes), val s1 = val s2 <=> s1 = s2
     by smt(@NBytes).
+
+(** -------------------------------------------------------------------------------------------- **)
+
+lemma simplify_pow (a b : int) : 
+    0 < a /\ 0 < b => 
+      a%r ^ b%r = (a ^ b)%r.
+proof.
+move => [#] ??.
+rewrite -RField.fromintXn 1:/# #smt:(@RealExp).
+qed.
+
+hint simplify simplify_pow. 
+
+lemma log2_16 : log2 16%r = 4%r.
+proof.
+have ->: 16%r = 2%r ^ 4%r by simplify.
+rewrite /log2 logK /#.
+qed.
+
+lemma ceil_3_2 : ceil (3%r / 2%r) = 2.
+proof.
+have ? : 1 < ceil (3%r / 2%r) by smt(@Real).
+have ? : ceil (3%r / 2%r) <= 2 by smt(@Real).
+smt().
+qed.
+
+(** -------------------------------------------------------------------------------------------- **)
+
+lemma array3_map_bounds (y : W32.t Array3.t) :
+    (forall (x : int), x \in map W32.to_uint (to_list y) => 0 <= x && x < w) =>
+    (forall (k : int), 0 <= k < 3 => 0 <= to_uint y.[k] < w).
+proof.
+move => E.
+have E0 : forall (k : int), 0 <= k < 3 => 0 <= nth witness (map W32.to_uint (to_list y)) k < w by smt(@List).
+move => k?.
+rewrite -get_to_list. 
+rewrite -(nth_map witness witness W32.to_uint). 
+  + by rewrite size_to_list. 
+apply E0 => //=. 
+qed.
